src/Init/Data/List/Erase.lean
@@ -57,14 +57,8 @@ theorem eraseP_of_forall_not {l : List α} (h : ∀ a, a ∈ l → ¬p a) : l.er
       rintro x h' rfl
       simp_all
 
-@[deprecated eraseP_eq_nil_iff (since := "2025-01-30")]
-abbrev eraseP_eq_nil := @eraseP_eq_nil_iff
-
 theorem eraseP_ne_nil_iff {xs : List α} {p : α → Bool} : xs.eraseP p ≠ [] ↔ xs ≠ [] ∧ ∀ x, p x → xs ≠ [x] := by
   simp
-
-@[deprecated eraseP_ne_nil_iff (since := "2025-01-30")]
-abbrev eraseP_ne_nil := @eraseP_ne_nil_iff
 
 theorem exists_of_eraseP : ∀ {l : List α} {a} (_ : a ∈ l) (_ : p a),
     ∃ a l₁ l₂, (∀ b ∈ l₁, ¬p b) ∧ p a ∧ l = l₁ ++ a :: l₂ ∧ l.eraseP p = l₁ ++ l₂
@@ -352,16 +346,10 @@ theorem erase_eq_eraseP [LawfulBEq α] (a : α) : ∀ (l : List α), l.erase a =
   rw [erase_eq_eraseP]
   simp
 
-@[deprecated erase_eq_nil_iff (since := "2025-01-30")]
-abbrev erase_eq_nil := @erase_eq_nil_iff
-
 theorem erase_ne_nil_iff [LawfulBEq α] {xs : List α} {a : α} :
     xs.erase a ≠ [] ↔ xs ≠ [] ∧ xs ≠ [a] := by
   rw [erase_eq_eraseP]
   simp
-
-@[deprecated erase_ne_nil_iff (since := "2025-01-30")]
-abbrev erase_ne_nil := @erase_ne_nil_iff
 
 theorem exists_erase_eq [LawfulBEq α] {a : α} {l : List α} (h : a ∈ l) :
     ∃ l₁ l₂, a ∉ l₁ ∧ l = l₁ ++ a :: l₂ ∧ l.erase a = l₁ ++ l₂ := by
@@ -591,8 +579,7 @@ theorem eraseIdx_ne_nil_iff {l : List α} {i : Nat} : eraseIdx l i ≠ [] ↔ 2 
   | [a]
   | a::b::l => simp
 
-@[deprecated eraseIdx_ne_nil_iff (since := "2025-01-30")]
-abbrev eraseIdx_ne_nil := @eraseIdx_ne_nil_iff
+
 
 @[grind]
 theorem eraseIdx_sublist : ∀ (l : List α) (k : Nat), eraseIdx l k <+ l
@@ -700,7 +687,6 @@ theorem erase_eq_eraseIdx_of_idxOf [BEq α] [LawfulBEq α]
     rw [eq_comm, eraseIdx_eq_self]
     exact Nat.le_of_eq (idxOf_eq_length h).symm
 
-@[deprecated erase_eq_eraseIdx_of_idxOf (since := "2025-01-29")]
-abbrev erase_eq_eraseIdx_of_indexOf := @erase_eq_eraseIdx_of_idxOf
+
 
 end List
